exercicios e novos materiais

Fad/Chapter3.lean
@@ -5,10 +5,39 @@ open List (reverse tail cons)
 
 -- 3.1 Symmetric lists
 
-def snoc {a : Type u} (x : a) (xs : List a) : List a :=
+def snoc {a : Type} (x : a) (xs : List a) : List a :=
   xs ++ [x]
 
 abbrev SymList (α : Type u) := (List α) × (List α)
+
+def single (xs : List α) : Prop := xs.length = 1
+
+structure SymList' (α : Type) where
+  lhs : List α
+  rhs : List α
+  ok : (lhs.isEmpty → rhs.isEmpty ∨ single rhs) ∧
+       (rhs.isEmpty → lhs.isEmpty ∨ single lhs)
+ deriving Repr
+
+#eval SymList'.mk [1,2,3] [4,5,6] (by
+  apply And.intro
+  { intro h; simp at h }
+  { intro h; simp at h })
+
+#eval { lhs := [1,2,3], rhs := [4,5,6], ok := (by
+  apply And.intro
+  { intro h; simp at h }
+  { intro h; simp at h }) : SymList' Nat }
+
+
+def P (sl : SymList' a) : Prop :=
+ sl.1.length > sl.2.length
+
+example : ∀ sl : SymList' Nat, P sl := by
+  intro sl
+  cases sl with
+  | mk as bs h => sorry
+
 
 #check ([],[])
 
@@ -57,8 +86,8 @@ def tailSL (sl : SymList a) : Option (SymList a) :=
 #eval tailSL (snocSL 1 (snocSL 2 (snocSL 3 ([], [])))) >>= pure ∘ fromSL
 
 
-/- Evidencias como argumentos
-https://lean-lang.org/functional_programming_in_lean/props-proofs-indexing.html#evidence-as-arguments
+/-
+ https://lean-lang.org/functional_programming_in_lean/props-proofs-indexing.html#evidence-as-arguments
 -/
 
 #check ([] : List Nat)
@@ -74,9 +103,9 @@ def mytest (n : Nat) := n
 def terceiro (xs : List α) (ok : xs.length > 2) : α := xs[2]
 #eval terceiro [1, 2, 3, 4] (by simp)
 
-
-example : cons x ∘ fromSL = fromSL ∘ consSL x := by
-  funext xs
+example
+  : cons x ∘ fromSL = fromSL ∘ consSL x := by
+  funext (as, bs)
   sorry
 
 /- pagina 45 provar a equacao -/
@@ -84,8 +113,7 @@ example : cons x ∘ fromSL = fromSL ∘ consSL x := by
 #eval reverse [4,5,6] ++ reverse [1,2,3]
 
 example (us vs : List Nat)
- : [] ++ reverse (us ++ vs) = reverse vs ++ reverse us := by
- sorry
+ : [] ++ reverse (us ++ vs) = reverse vs ++ reverse us := by simp
 
 
 -- 3.2 Random-access lists
@@ -103,6 +131,13 @@ inductive Tree (α : Type) : Type where
  | node (n : Nat) (t₁ : Tree α) (t₂ : Tree α) : Tree α
  deriving Repr
 
+def Tree.toString [ToString α] : Tree α → String
+ | leaf x => s!"leaf {x}"
+ | node n t₁ t₂ => s!"node {n} ({t₁.toString}) ({t₂.toString})"
+
+instance [ToString α] : ToString (Tree α) where
+  toString := Tree.toString
+
 def Tree.size : Tree a → Nat
  | leaf _ => 1
  | node n _ _ => n
@@ -110,13 +145,23 @@ def Tree.size : Tree a → Nat
 def Tree.mk (t₁ t₂ : Tree a) : Tree a :=
  node (t₁.size + t₂.size) t₁ t₂
 
-open Tree in
+open Tree
+
 #eval mk (mk (leaf 'a') (leaf 'b')) (mk (leaf 'c') (leaf 'd'))
 
 inductive Digit (a : Type) : Type where
  | zero : Digit a
  | one (t : Tree a) : Digit a
  deriving Repr
+
+def Digit.toString [ToString α] : Digit α → String
+  | zero => "zero"
+  | one t => s!"one ({t.toString})"
+
+instance [ToString α] : ToString (Digit α) where
+  toString := Digit.toString
+
+open Digit
 
 -- works with def too
 abbrev RAList (a : Type) : Type := List (Digit a)
@@ -129,7 +174,7 @@ def concat1 {a : Type} : List (List a) → List a :=
 def concatMap (f : a → List b) : List a → List b :=
  concat1 ∘ (List.map f)
 
-open Tree in
+
 def fromT : Tree a → List a
  | (leaf x) => [x]
  | (node _ t₁ t₂) => fromT t₁ ++ fromT t₂
@@ -141,10 +186,31 @@ def fromRA : RAList a → List a :=
    | Digit.zero => []
    | Digit.one t => fromT t
 
-open Tree in
-open Digit in
-
 #eval fromRA [zero,
+        one (mk (leaf 'a') (leaf 'b')),
+        one (mk (mk (leaf 'c') (leaf 'd'))
+                (mk (leaf 'e') (leaf 'f')))]
+
+
+def fetchT [ToString a] (n : Nat) (t : Tree a) : Option a :=
+ dbg_trace "fetchT {n} {t.toString}"
+ match n, t with
+ | 0, leaf x => some x
+ | k, (node n t₁ t₂) =>
+   let m := n / 2
+   if k < m
+   then fetchT k t₁ else fetchT (k - m) t₂
+ | _, leaf _ => none
+
+def fetchRA [ToString a] (n : Nat) (ra : RAList a) : Option a :=
+ dbg_trace "fetchRA {n} {ra.toString}"
+ match n, ra with
+ | _, [] => none
+ | k, (zero :: xs) => fetchRA k xs
+ | k, (one t :: xs) =>
+   if k < size t then fetchT k t else fetchRA (k - size t) xs
+
+#eval fetchRA 10 [zero,
         one (mk (leaf 'a') (leaf 'b')),
         one (mk (mk (leaf 'c') (leaf 'd'))
                 (mk (leaf 'e') (leaf 'f')))]
