Fad/Chapter1-Ex.lean
@@ -63,7 +63,6 @@ example : ∀ xs : List Nat, single xs = true ↔ xs.length = 1 := by
     rw [single_aux]
     simp [List.length]
 
-
 def reverse {α : Type} (a : List α) : List α :=
   let rec helper (a : List α) (res : List α) : List α :=
     match a with
@@ -74,6 +73,8 @@ def reverse {α : Type} (a : List α) : List α :=
 example : reverse [3, 4, 5] = [5, 4, 3] := rfl
 example : reverse ([] : List Nat) = [] := rfl
 
+example (xs : List Nat): reverse (reverse xs) = xs := by
+  sorry
 
 example (f : α → β → β) :
  (foldr f e) ∘ (filter p) = foldr (λ x y => if p x then f x y else y) e
@@ -101,6 +102,16 @@ example (f : α → β → α) : map (foldl f e) ∘ inits = scanl f e := sorry
 
 example (f : α → β → β) : map (foldr f e) ∘ tails = scanr f e := sorry
 
+def steep₀ (xs : List Nat) : Bool :=
+  let sum (xs : List Nat) : Nat :=
+    xs.foldl (· + ·) 0
+  match xs with
+  | []  => true
+  | x :: xs => x > sum xs ∧ steep₀ xs
+
+set_option trace.profiler true
+
+#eval steep₀ (List.iota 10000000)
 
 def steep₁ (xs : List Nat) : Bool :=
   let rec sum : List Nat → Nat
@@ -110,6 +121,7 @@ def steep₁ (xs : List Nat) : Bool :=
   | []  => true
   | x :: xs => x > sum xs ∧ steep₁ xs
 
+#eval steep₁ [2,0]
 
 def steep₂ : List Nat → Bool :=
  Prod.snd ∘ faststeep
@@ -119,6 +131,15 @@ def steep₂ : List Nat → Bool :=
   | x :: xs =>
     let (s, b) := faststeep xs
     (x + s, x > s ∧ b)
+
+def steep₃ : List Nat → Bool :=
+ Prod.snd ∘ faststeep
+ where
+  faststeep (xs : List Nat) : (Nat × Bool) :=
+   xs.reverse.foldl (λ t x => (x + t.1, x > t.1 ∧ t.2) ) (0, true)
+
+#eval steep₃ [8,5,2]
+#eval steep₃ (List.range 100000)
 
 example : steep₁ [8,4,2,1] = steep₂ [8,4,2,1] := rfl
 example : steep₁ [] = steep₂ [] := rfl
